Complete taint analysis

src/arch/x64/X64.Leakage_Helpers_i.fst
@@ -4,14 +4,38 @@ open X64.Machine_s
 open X64.Taint_Semantics_s
 open X64.Leakage_s
 
+val publicFlagValuesAreAsExpected: (tsAnalysis:taintState) -> (tsExpected:taintState) -> b:bool{b <==> (Public? tsExpected.flagsTaint ==> Public? tsAnalysis.flagsTaint)}
+
+val publicRegisterValuesAreAsExpected: (tsAnalysis:taintState) -> (tsExpected:taintState) -> b:bool{b <==> (forall r. (Public? (tsExpected.regTaint r) ==> Public? (tsAnalysis.regTaint r)))}
+
+val publicTaintsAreAsExpected: (tsAnalysis:taintState) -> (tsExpected:taintState) -> b:bool
+
 let publicFlagValuesAreAsExpected (tsAnalysis:taintState) (tsExpected:taintState) =
-  tsExpected.flagsTaint == Public ==> tsAnalysis.flagsTaint == Public
+  (tsExpected.flagsTaint = Public && tsAnalysis.flagsTaint = Public) || (tsExpected.flagsTaint = Secret)
+
+let registerAsExpected (r:reg) (tsAnalysis:taintState) (tsExpected:taintState) =
+  (tsExpected.regTaint r = Public && tsAnalysis.regTaint r = Public) || (tsExpected.regTaint r = Secret)
 
 let publicRegisterValuesAreAsExpected (tsAnalysis:taintState) (tsExpected:taintState) =
-  forall r. (tsExpected.regTaint r = Public) ==> (tsAnalysis.regTaint r = Public)
+  registerAsExpected Rax tsAnalysis tsExpected &&
+  registerAsExpected Rbx tsAnalysis tsExpected &&
+  registerAsExpected Rcx tsAnalysis tsExpected &&
+  registerAsExpected Rdx tsAnalysis tsExpected &&
+  registerAsExpected Rsi tsAnalysis tsExpected &&
+  registerAsExpected Rdi tsAnalysis tsExpected &&
+  registerAsExpected Rbp tsAnalysis tsExpected &&
+  registerAsExpected Rsp tsAnalysis tsExpected &&
+  registerAsExpected R8 tsAnalysis tsExpected &&
+  registerAsExpected R9 tsAnalysis tsExpected &&
+  registerAsExpected R10 tsAnalysis tsExpected &&
+  registerAsExpected R11 tsAnalysis tsExpected &&
+  registerAsExpected R12 tsAnalysis tsExpected &&
+  registerAsExpected R13 tsAnalysis tsExpected &&
+  registerAsExpected R14 tsAnalysis tsExpected &&
+  registerAsExpected R15 tsAnalysis tsExpected
 
 let publicTaintsAreAsExpected (tsAnalysis:taintState) (tsExpected:taintState) =
     publicFlagValuesAreAsExpected tsAnalysis tsExpected
-  /\ publicRegisterValuesAreAsExpected tsAnalysis tsExpected
+  && publicRegisterValuesAreAsExpected tsAnalysis tsExpected
 
 
